Foundation/FirstOrder/Arithmetic/ISigma1/Prenex.lean
@@ -16,22 +16,23 @@ open LO.FirstOrder
 
 namespace LO.FirstOrder.Arithmetic.ISigma1
 
-variable {n : ℕ}
+variable {n : ℕ} {φ : ArithmeticSemisentence n} {σ : ArithmeticSentence}
 
-lemma nonempty_prenexNormalForm {φ : ArithmeticSemisentence n} (h : Hierarchy 𝚺 1 φ) :
-    Nonempty (ArithmeticSemisentence.PrenexNormalForm 𝗜𝚺₁ 𝚺 1 φ) :=
-  Arithmetic.nonempty_prenexNormalForm h
+lemma hasPrenex (h : Hierarchy 𝚺 1 φ) :
+    ∃ π : Prenex 𝚺 1 Empty n, 𝗜𝚺₁ ⊢ ∀¹* (φ 🡘 π.val) :=
+  Arithmetic.hasPrenex h
 
-lemma exists_matrix_provable {φ : ArithmeticSemisentence n} (h : Hierarchy 𝚺 1 φ) :
+lemma exists_matrix_provable (h : Hierarchy 𝚺 1 φ) :
     ∃ θ : ArithmeticSemisentence (n + 1), Hierarchy 𝚺 0 θ ∧ 𝗜𝚺₁ ⊢ ∀¹* (φ 🡘 ∃¹ θ) := by
-  obtain ⟨φ'⟩ := nonempty_prenexNormalForm h;
-  exact ⟨↑φ'.sigmaInv, φ'.sigmaInv.deltaZero, φ'.provable_sigmaInv⟩
+  obtain ⟨π, hπ⟩ := hasPrenex h;
+  exact ⟨π.sigmaInv.val, π.sigmaInv.val_deltaZero, Prenex.provable_iff_sigmaInv hπ⟩
 
-lemma exists_matrix_provable_pi {φ : ArithmeticSemisentence n} (h : Hierarchy 𝚷 1 φ) :
-    ∃ θ : ArithmeticSemisentence (n + 1), Hierarchy 𝚺 0 θ ∧ 𝗜𝚺₁ ⊢ ∀¹* (φ 🡘 ∀¹ θ) :=
-  Arithmetic.exists_matrix_provable _ h
+lemma exists_matrix_provable_pi (h : Hierarchy 𝚷 1 φ) :
+    ∃ θ : ArithmeticSemisentence (n + 1), Hierarchy 𝚺 0 θ ∧ 𝗜𝚺₁ ⊢ ∀¹* (φ 🡘 ∀¹ θ) := by
+  obtain ⟨π, hπ⟩ := Arithmetic.hasPrenex (T := 𝗜𝚺₁) h
+  exact ⟨π.piInv.val, π.piInv.val_hierarchy, Prenex.provable_iff_piInv hπ⟩
 
-lemma exists_matrix_provable_of_sentence {σ : ArithmeticSentence} (h : Hierarchy 𝚺 1 σ) :
+lemma exists_matrix_provable_of_sentence (h : Hierarchy 𝚺 1 σ) :
     ∃ θ : ArithmeticSemisentence 1, Hierarchy 𝚺 0 θ ∧ 𝗜𝚺₁ ⊢ σ 🡘 ∃¹ θ :=
   exists_matrix_provable h
 
